cedar-dafny/pe/soundness.dfy
@@ -15,7 +15,7 @@ module pe.soundness {
   import def.base
   import opened def.std
 
-  lemma makeErrorValueIsErr(env: Environment)
+  lemma MakeErrorValueIsErr(env: Environment)
     requires env.wellFormed()
     ensures var r := PartialEvaluator.makeErrorValue(); env.interpret(r, core.EntityStore(map[])).Err? {
     calc {
@@ -30,9 +30,60 @@ module pe.soundness {
     }
   }
 
-  lemma PEIsSoundGetAttr(e: definition.Expr, q: core.Request, s: core.EntityStore, Q: definition.Request, S: definition.EntityStore, env: Environment)
+  lemma InterpretRestrictedResidualSet(rs: seq<Residual>, env: Environment, s: core.EntityStore)
+    requires forall r | r in rs :: r.restricted?()
     requires env.wellFormed()
-    requires e.GetAttr?
+    ensures env.interpretSet(rs, s) == env.interpretSet(rs, core.EntityStore(map[]))
+  {
+    if |rs| == 0 {
+
+    } else {
+      InterpretRestrictedResidual(rs[0], env, s);
+    }
+  }
+
+  lemma InterpretRestrictedResidualRecord(bs: seq<(core.Attr, Residual)>, env: Environment, s: core.EntityStore)
+    requires forall b | b in bs :: b.1.restricted?()
+    requires env.wellFormed()
+    ensures env.interpretRecord(bs, s) == env.interpretRecord(bs, core.EntityStore(map[]))
+  {
+    if |bs| == 0 {
+
+    } else {
+      InterpretRestrictedResidual(bs[0].1, env, s);
+    }
+  }
+
+  lemma InterpretRestrictedResidualList(rs: seq<Residual>, env: Environment, s: core.EntityStore)
+    requires forall r | r in rs :: r.restricted?()
+    requires env.wellFormed()
+    ensures env.interpretList(rs, s) == env.interpretList(rs, core.EntityStore(map[])) {
+    if |rs| == 0 {
+
+    } else {
+      InterpretRestrictedResidual(rs[0], env, s);
+    }
+  }
+
+  lemma InterpretRestrictedResidual(r: Residual, env: Environment, s: core.EntityStore)
+    requires r.restricted?()
+    requires env.wellFormed()
+    ensures env.interpret(r, s) == env.interpret(r, core.EntityStore(map[]))
+  {
+    match r {
+      case Concrete(_) =>
+      case Unknown(_) =>
+      case Set(rs) => InterpretRestrictedResidualSet(rs, env, s);
+      case Record(bs) => InterpretRestrictedResidualRecord(bs, env, s);
+      case Call(_, args) => InterpretRestrictedResidualList(args, env, s);
+      case _ => assume false;
+    }
+  }
+
+  lemma PEIsSoundSet(e: definition.Expr, q: core.Request, s: core.EntityStore, Q: definition.Request, S: definition.EntityStore, env: Environment)
+    requires env.wellFormed()
+    requires restrictedEntityStore(S)
+    requires e.Set?
     // Request is well formed
     requires var pr := env.replaceUnknownInRequest(Q); pr.Some? && pr.value == q
     // Entity store is well formed
@@ -41,55 +92,30 @@ module pe.soundness {
             // If PE succeeds, then evaluating the residual and evaluating the original expression with the same unknown to value mappings should agree.
             (peRes.Ok? ==> ce.Evaluator(q, s).interpret(env.replaceUnknownInExpr(e)) == env.interpret(peRes.value, s)) &&
             // If PE fails, then evaluating the original expression with any uknown to value mappings should fail.
-            (peRes.Err? ==> ce.Evaluator(q, s).interpret(env.replaceUnknownInExpr(e)).Err?) {
+            (peRes.Err? ==> ce.Evaluator(q, s).interpret(env.replaceUnknownInExpr(e)).Err?)
+  {
     var peRes := PartialEvaluator(Q, S).interpret(e);
     match e {
-
-      case GetAttr(se, a) =>
-        var peRes' := PartialEvaluator(Q, S).interpret(se);
-        PEIsSound(se, q, s, Q, S, env);
-        if peRes'.Err? {
-
-        } else {
-          var peVal' := peRes'.value;
-          if peVal'.Concrete? {
-            var concreteVal' := peVal'.v;
-            match concreteVal' {
-              case Primitive(EntityUID(euid)) =>
-                if euid in s.entities.Keys {
-                  if a in s.entities[euid].attrs.Keys {
-                    calc == {
-                      ce.Evaluator(q, s).interpret(env.replaceUnknownInExpr(e));
-                      Ok(s.entities[euid].attrs[a]);
-                    }
-                    calc == {
-                      peRes;
-                      Ok(S.entities[euid].attrs[a]);
-                    }
-                    assume env.interpret(S.entities[euid].attrs[a], s).Ok? && env.interpret(S.entities[euid].attrs[a], s).value == s.entities[euid].attrs[a];
-                    //calc == {
-                    //  env.interpret(peRes.value, s);
-                    //  Ok(s.entities[euid].attrs[a]);
-                    //}
-                  } else {
-
-                  }
-
-
-                } else {
-                }
-              case _ =>
-
-            }
+      case Set(es) =>
+        forall e' | e' in es {
+          PEIsSound(e', q, s, Q, S, env);
+        }
+        var rs := PartialEvaluator(Q, S).interpretSeq(es);
+        if rs.Ok? {
+          if (forall r | r in rs.value :: r.Concrete?) {
+            assume false;
           } else {
-
+            assume false;
           }
+        } else {
+          assume false;
         }
     }
   }
 
   lemma PEIsSound(e: definition.Expr, q: core.Request, s: core.EntityStore, Q: definition.Request, S: definition.EntityStore, env: Environment)
     requires env.wellFormed()
+    requires restrictedEntityStore(S)
     // Request is well formed
     requires var pr := env.replaceUnknownInRequest(Q); pr.Some? && pr.value == q
     // Entity store is well formed
@@ -124,6 +150,28 @@ module pe.soundness {
       case BinaryApp(op, arg1, arg2) =>
         PEIsSound(arg1, q, s, Q, S, env);
         PEIsSound(arg2, q, s, Q, S, env);
+      case GetAttr(se, a) =>
+        var peRes' := PartialEvaluator(Q, S).interpret(se);
+        PEIsSound(se, q, s, Q, S, env);
+        if peRes'.Ok? {
+          var peVal' := peRes'.value;
+          if peVal'.Concrete? {
+            var concreteVal' := peVal'.v;
+            match concreteVal' {
+              case Primitive(EntityUID(euid)) =>
+                if euid in s.entities.Keys {
+                  if a in s.entities[euid].attrs.Keys {
+                    assert restrictedEntityData(S.entities[euid]);
+                    InterpretRestrictedResidual(S.entities[euid].attrs[a], env, s);
+                  }
+                }
+              case _ =>
+            }
+          }
+        }
+      case HasAttr(se, a) =>
+        PEIsSound(se, q, s, Q, S, env);
+      case Set(es) => assume false;
       case _ => assume false;
     }
   }
